Update automata.lean

scripts/automata.lean
@@ -1,71 +1,133 @@
 
 /- Ch. 1 of "Intro. to Theory of Computation" (3rd ed.) by Sipser -/
 
-def subset (X: Type): Type := X → Prop
+-- sets 
+def subset (X: Type): Type :=
+  X → Prop
 
-structure FiniteAutomaton (alphabet: Type) where
+def singleton {X: Type} (x0: X): subset X :=
+  fun x => x = x0
+
+-- automata
+
+structure FinAutomaton (α: Type) where
   state: Type
-  transition: state × alphabet → state
+  transition: state → α → state
   initial: state
   final: subset state
 
-def run (M: FiniteAutomaton A) (string: List A): M.state :=
-  string.foldl (fun s a => M.transition (s, a)) M.initial
+def run (M: FinAutomaton α) (string: List α): M.state :=
+  match string with
+  | [] => M.initial
+  | head :: tail => M.transition (run M tail) head
 
-def accept (M: FiniteAutomaton A) (string: List A): Prop :=
-  M.final (run M string)
+def accept (M: FinAutomaton α) (string: List α): Prop :=
+  let state := run M string
+  M.final state
 
-def reject (M: FiniteAutomaton A) (string: List A): Prop :=
-  ¬ (accept M string)
+def reject (M: FinAutomaton α) (string: List α): Prop :=
+  ¬(accept M string)
 
-def language_of (M: FiniteAutomaton A): subset (List A) :=
-  fun string => accept M string
-
-def Language (alphabet: Type): Type := subset (List alphabet)
-
-def regular (L: Language A): Prop :=
-  ∃ M: FiniteAutomaton A, language_of M = L
-
-/- define the union, concatenation, and star of languages -/
-def union (L1: Language A1) (L2: Language A2): Language (Sum A1 A2) :=
-  fun string => sorry
-
-def concat (L1: Language A1) (L2: Language A2): Language (Sum A1 A2) :=
-  fun string => sorry
-
-def star (L: Language A): Language (List A) :=
-  fun string => sorry
-
-def star2 (L: Language A): Language A :=
-  fun string => sorry
-
-structure NondeterministicFiniteAutomaton (alphabet: Type) where
+structure NondetFinAutomaton (α: Type) where
   state: Type
-  transition: state × alphabet → subset state
+  transition: state → α → subset state
   initial: state
   final: subset state
 
-def NFA.run (M: NondeterministicFiniteAutomaton A) (string: List A): subset M.state :=
-  sorry
+def NFA.run (M: NondetFinAutomaton α) (string: List α): subset M.state :=
+  match string with
+  | [] => singleton M.initial
+  | head :: tail => sorry
 
-def NFA.accept (M: NondeterministicFiniteAutomaton A) (string: List A): Prop :=
+def NFA.accept (M: NondetFinAutomaton α) (string: List α): Prop :=
   ∃ s: M.state, (NFA.run M string) s ∧ M.final s
 
-def NFA.reject (M: NondeterministicFiniteAutomaton A) (string: List A): Prop :=
-  ¬ (NFA.accept M string)
+def NFA.reject (M: NondetFinAutomaton α) (string: List α): Prop :=
+  Not (NFA.accept M string)
 
-def NFA.language_of (M: NondeterministicFiniteAutomaton A): subset (List A) :=
+def NFA.language_of (M: NondetFinAutomaton α): subset (List α) :=
   fun string => NFA.accept M string
 
-theorem equivalence (M: NondeterministicFiniteAutomaton A): ∃ M': FiniteAutomaton A, NFA.language_of M = language_of M' := sorry
+-- languages
 
-theorem corollary (L: Language A): regular L ↔ ∃ M: NondeterministicFiniteAutomaton A, NFA.language_of M = L := sorry
+def Language (α: Type): Type := subset (List α)
 
-/- next prove regular language are closed under all these -/
-theorem union_of_regular_is_regular (L1: Language A1) (L2: Language A2) (h1: regular L1) (h2: regular L2): regular (union L1 L2) := sorry
+def language_of (M: FinAutomaton α): Language α :=
+  fun string => accept M string
 
-theorem concat_of_regular_is_regular (L1: Language A1) (L2: Language A2) (h1: regular L1) (h2: regular L2): regular (concat L1 L2) := sorry
+def regular (L: Language α): Prop :=
+  ∃ M: FinAutomaton α, language_of M = L
 
-theorem star_of_regular_is_regular (L: Language A) (h: regular L): regular (star L) := sorry
+theorem equivalence (M: NondetFinAutomaton α): ∃ M': FinAutomaton α, NFA.language_of M = language_of M' := by
+  sorry
+
+theorem corollary (L: Language α): regular L ↔ ∃ M: NondetFinAutomaton α, NFA.language_of M = L := by
+  sorry
+
+-- helpers
+def all_left: List (Sum α0 α1) → Prop
+  | [] => True
+  | (Sum.inl _) :: tail => all_left tail
+  | (Sum.inr _) :: _ => False
+
+def all_right: List (Sum α0 α1) → Prop
+  | [] => True
+  | (Sum.inl _) :: tail => all_right tail
+  | (Sum.inr _) :: _ => False
+
+def convert_left: List (Sum α0 α1) → List α0
+  | [] => []
+  | (Sum.inl head) :: tail => head :: convert_left tail
+  | (Sum.inr _) :: tail => convert_left tail
+
+def convert_right: List (Sum α0 α1) → List α1
+  | [] => []
+  | (Sum.inl _) :: tail => convert_right tail
+  | (Sum.inr head) :: tail => head :: convert_right tail
+
+/- union, concatenation, and star of languages -/
+def union (L0: Language α0) (L1: Language α1): Language (Sum α0 α1) :=
+  fun string => (all_left string ∧ L0 (convert_left string)) ∨ (all_right string ∧ L1 (convert_right string))
+
+def concat (L0: Language α0) (L1: Language α1): Language (Sum α0 α1) :=
+  fun string => ∃ x y: List (Sum α0 α1), (string = List.append x y) ∧ (all_left x) ∧ (all_right y) ∧ L0 (convert_left x) ∧ L1 (convert_right y)
+
+def collapse (L: List (List α)): List α :=
+  match L with
+  | [] => []
+  | head :: tail => List.append (collapse tail) head
+
+def star (L: Language α): Language (List α) :=
+  fun string => L (collapse string)
+
+def star2 (L: Language α): Language α :=
+  fun string => ∃ Ls: List (List α), (collapse Ls = string) ∧ (∀ x ∈ Ls, L x)
+
+theorem union_of_regular_is_regular (L0: Language α0) (L1: Language α1): regular L0 ∧ regular L1 -> regular (union L0 L1) := by
+  intro ⟨L0_regular, L1_regular⟩
+  -- let M1 and M2 be the corresponding automata
+  obtain ⟨M0, h0⟩ := L0_regular
+  obtain ⟨M1, h1⟩ := L1_regular 
+  -- now construct an automaton to recognize the union
+  let M : FinAutomaton (Sum α0 α1) := {
+    state := M0.state × M1.state
+    transition := fun (s0, s1) => fun a => match a with
+    | Sum.inl a => (M0.transition s0 a, s1)
+    | Sum.inr a => (s0, M1.transition s1 a)
+    initial := (M0.initial, M1.initial)
+    final := fun (s0, s1) => (M0.final s0) ∨ (M1.final s1)
+  }
+  exists M
+  apply funext
+  intro string
+  rw [language_of, union]
+  -- ?? seems to be a problem here
+  sorry
+
+theorem concat_of_regular_is_regular (L0: Language α0) (L1: Language α1): (regular L0) ∧ (regular L1) -> regular (concat L0 L1) := by
+  sorry
+
+theorem star_of_regular_is_regular (L: Language α): regular L -> regular (star L) := by
+  sorry
 
 /- todo: regular expressions and pumping lemma -/
